doc/ExampleInspect.fst
@@ -11,10 +11,24 @@ let show_an_arrow_expr () : Tac unit =
 let addition : int -> int -> int = synth_by_tactic show_an_arrow_expr
 
 let show_term _ : Tac unit = 
+  print "Term 1\n";
   let t = (`(fun (z:int) -> z)) in
     print (term_to_ast_string t);
+  print "Term 2\n";
   let t2 = (`(fun (z:int{z<2}) -> z)) in
     print (term_to_ast_string t2);
+  print "Term 3\n";
+  let t3 = (`(let rec f (x:nat) : nat = if x = 0 then 2 else 3 + f (x - 1) in f(5))) in
+    print (term_to_ast_string t3);
+  print "Term 4\n";
+  let t4 = (`(let f (x:nat) : Lemma( x + 1 = 1 + x ) = () in f)) in
+    print (term_to_ast_string t4);
+  print "Term 5\n";
+  let t5 = (`((x:nat) -> Lemma( x + 1 = 1 + x ))) in
+    print (term_to_ast_string t5);
+  print "Term 5\n";
+  let t5 = (`((x:nat) -> Lemma( x + 1 = 1 + x ))) in
+    print (term_to_ast_string t5);
   exact (quote 1)
 
 let foo : int = synth_by_tactic show_term
