doc/ExampleInduction.fst
@@ -1,0 +1,87 @@
+module ExampleInduction
+
+open FStar.Mul
+open FStar.Tactics
+
+(*
+Show use of tactics to prove an assertion via induction.
+*)
+
+// Example functions we might want to prove things about
+val factorial: nat -> Tot int
+let rec factorial n = 
+  if n = 0 then 1 else n * (factorial (n - 1))
+
+let rec sum_of_squares (x:nat) : Tot int =
+  if x = 0 then 0 else (x * x) + (sum_of_squares (x-1) )
+  
+// Our super-powerful metatheorem about induction on natural numbers.
+let rec nat_induction (p : nat -> Type) (n:nat)
+  : Lemma (requires p 0 /\ (forall (x:nat) . ( x > 0 /\ p (x-1) ) ==> p x ))
+    (ensures p n)
+  = if n = 0 then () else nat_induction p (n-1)
+
+// Unwrap a term that has been squashed
+// Perhaps we could just use (unsquash (pack t))?
+let access_type_in_squash (t:typ) : Tac term =
+  match inspect t with 
+  | Tv_App hd a -> 
+    begin
+    match inspect hd with
+    | Tv_FVar f ->
+       if inspect_fv f = squash_qn then
+          fst a
+       else
+          fail "Not a squash type"
+    | _ -> fail "Not a squash type"
+    end
+  | _ -> fail "Not a squash type"
+
+// Check that there is just one binder in the current
+// environment, and reutrn it.
+let induction_binder () : Tac binder =
+  match cur_binders() with
+  | [] -> fail "No variable in environment"
+  | hd :: [] -> hd
+  | hd :: tl -> fail "More than one variable in environment"
+
+// Paste together the current binder and the current (unsquashed) goal
+// to get the abstraction we need to use `nat_induction`.
+// Frankly, I am not sure how we got away with this; not recommended for production use.
+let nat_induction_tac () : Tac unit =
+     let term_to_prove = access_type_in_squash (cur_goal()) in (
+       print ("goal type = " ^ term_to_string( term_to_prove ) );
+       let binder = induction_binder() in
+         print ("binder = " ^ binder_to_string( binder) );
+           let myProp = mk_abs [binder] term_to_prove in
+             let l = mk_e_app (`nat_induction) [myProp] in
+               print( "my_lemma = " ^ term_to_string( l ) );
+               dump "before";
+               apply_lemma l;
+               dump "after lemma";
+               split();
+               dump "after split"
+     )
+
+let factorial_is_positive (n:nat) = 
+  assert (factorial n > 0) by nat_induction_tac()
+
+let factorial_is_greater_than_arg (n:nat) = 
+  assert (factorial n >= n) by nat_induction_tac()
+
+let sum_of_squares_formula (m:nat) = 
+  assert (sum_of_squares m = (2*m+1)*m*(m+1)/6) by nat_induction_tac()
+
+(*
+Notes on failed approaches:
+
+We can't drop an antiquote in the middle of Lemma(), there's a check in the grammar that specifically prohibits that.
+We also can't put it in GTot(u:unit{...}).
+
+But, confusingly, the return type of a letrec is not part of the view?
+
+Computation types are part of sgelts view, but it looks like we can only introduce those if building a plugin?
+
+Can we define a type instead?  Not clear how to add type annotations, do they desugar to something?
+i.e., (let type = <blah> in let rec foo (x:nat) (Lemma type) = ... )
+*)
