doc/ExampleLogic.fst
@@ -1,0 +1,38 @@
+module ExampleLogic
+
+open FStar.Mul
+
+val factorial: n:nat -> Tot int
+let rec factorial n = 
+  if n = 0 then 1 else n * (factorial (n - 1))
+
+
+// Write the inductive proof as a logical statement
+
+// SMT can solve base case and inductive step
+let _ = assert( forall (y:nat) . 
+    ( ( y = 0 == true ) ==> (factorial 0 > 0 == true ) )
+    /\
+    ( ~(y = 0 == true) ==> (factorial (y-1) > 0 == true  ==> factorial y > 0 == true) ) )
+
+
+// But fails on induction
+[@@expect_failure]
+let _ = assert ( 
+    (  (factorial 0 > 0 == true )
+        /\
+        ( forall (y:nat) . ( (y > 0 == true) ==> (y -1 << y /\ (factorial (y-1) > 0 == true  ==> factorial y > 0 == true )))))
+     ==>
+    (forall (z:nat) . (factorial z > 0)))
+
+[@@expect_failure]
+let half_induction (n:nat) : Lemma
+  (requires (n == 0) ==> (factorial 0 > 0 == true ) /\
+            (n > 0 ) ==> (factorial (n-1) > 0 == true ==> factorial n > 0 == true))
+  (ensures (factorial n > 0))
+  = ()
+  
+let rec full_induction (n:nat) (p : nat -> prop) 
+  : Lemma (requires p 0 /\ (forall (x:nat) . ( x > 0 /\ p (x-1) ) ==> p x ))
+    (ensures p n)
+  = if n = 0 then () else full_induction (n-1) p
